Hoare Logic added

Tool/Semantics.thy
@@ -42,19 +42,7 @@ declare heap_update_def[simp]
 interpretation partial_comm_monoid map_add ortho Map.empty
   by default (auto simp: ortho_def intro: map_add_comm)
 
-(* Predicates about heaps *)
-definition is_singleton :: "nat \<Rightarrow> nat \<Rightarrow> heap \<Rightarrow> bool" where
-  "is_singleton e t h \<equiv> h = [e \<mapsto> t]"
-
-definition ex_singleton :: "nat \<Rightarrow> heap \<Rightarrow> bool" where
-  "ex_singleton e h \<equiv> \<exists>t. is_singleton e t h"
-
-primrec heap_by_list :: "nat \<Rightarrow> nat list \<Rightarrow> heap \<Rightarrow> bool" where
-  "heap_by_list e [] h \<longleftrightarrow> h = empty"
-| "heap_by_list e (t#ts) h \<longleftrightarrow> (\<exists>h1 h2. is_singleton e t h1 \<and> heap_by_list (Suc e) ts h2 \<and> h = h1++h2 \<and> (h1 \<bottom> h2))"
-
-
-section {* Assertion *}
+section {* Predicates *}
 
 definition emp :: "'a pred" where "emp \<equiv> \<lambda>(s, h). h = Map.empty"
 
@@ -107,6 +95,16 @@ lemma magic_wand_eq: "P -* Q = (\<lambda>(s, h). \<forall>h'. h' \<bottom> h \<a
   apply simp
   sorry
   
+(* Predicates about heaps *)
+definition is_singleton :: "nat \<Rightarrow> nat \<Rightarrow> heap \<Rightarrow> bool" where
+  "is_singleton e t h \<equiv> h = [e \<mapsto> t]"
+
+definition ex_singleton :: "nat \<Rightarrow> heap \<Rightarrow> bool" where
+  "ex_singleton e h \<equiv> \<exists>t. is_singleton e t h"
+
+primrec is_heap_list :: "nat \<Rightarrow> nat list \<Rightarrow> 'a pred" where
+  "is_heap_list e [] = emp"
+| "is_heap_list e (t#ts) = (\<lambda>(s, h). is_singleton e t h) * is_heap_list (Suc e) ts"
 
 section {* Predicate Transformers *}
 
@@ -127,13 +125,13 @@ interpretation PT: quantale_Sup_unital id "op o" Inf Sup inf less_eq less sup bo
   (* nitpick *) oops
 
 
-section {* Explicitly lifting between types *}
+section {* Lifting between types *}
 
 definition lift_stateT_pred :: "'a stateT \<Rightarrow> 'a state_predT" where
   "lift_stateT_pred f \<equiv> \<lambda>\<sigma> \<sigma>'. \<sigma>' = f \<sigma>"
 
 definition lift_state_pred_predT :: "'a state_predT \<Rightarrow> 'a predT" where
-  "lift_state_pred_predT F \<equiv> \<lambda>Q \<sigma>. \<forall>\<sigma>'. F \<sigma> \<sigma>' \<longrightarrow> Q \<sigma>'"
+  "lift_state_pred_predT F \<equiv> \<lambda>Q \<sigma>. F \<sigma> \<le> Q"
 
 definition lift_state_a_stateT :: "('a state \<Rightarrow> 'a) \<Rightarrow> 'a stateT" where
   "lift_state_a_stateT F \<equiv> \<lambda>(s, h). (F (s, h), h)"
@@ -142,7 +140,7 @@ definition lift_state_heap_stateT :: "('a state \<Rightarrow> heap) \<Rightarrow
   "lift_state_heap_stateT F \<equiv> \<lambda>(s, h). (s, F (s, h))"
 
 definition lift_stateT_predT :: "'a stateT \<Rightarrow> 'a predT" ("<_>") where
-  "<f> \<equiv> \<lambda>Q \<sigma>. \<forall>\<sigma>'. \<sigma>' = f \<sigma> \<longrightarrow> Q \<sigma>'"
+  "<f> \<equiv> \<lambda>Q. Q o f"
 
 definition lift_state_a_predT :: "('a state \<Rightarrow> 'a) \<Rightarrow> 'a predT" where
   "lift_state_a_predT F \<equiv> < lift_state_a_stateT F >"
@@ -151,7 +149,7 @@ definition lift_state_heap_predT :: "('a state \<Rightarrow> heap) \<Rightarrow>
   "lift_state_heap_predT F \<equiv> < lift_state_heap_stateT F >"
 
 definition lift_pred_predT :: "'a pred \<Rightarrow> 'a predT" ("\<lceil>_\<rceil>") where
-  "\<lceil>P\<rceil> \<equiv> \<lambda>Q s. P s \<longrightarrow> Q s"
+  "\<lceil>P\<rceil> \<equiv> \<lambda>Q. - P \<squnion> Q"
 
 declare lift_state_a_predT_def [simp]
   lift_state_heap_predT_def [simp]
@@ -166,7 +164,7 @@ abbreviation skip :: "'a predT" ("skip") where "skip \<equiv> id"
 
 notation comp (infixl ";" 60)
 
-abbreviation iteration :: "'a predT \<Rightarrow> 'a predT" ("_\<^sup>\<star>" [999] 1000) where
+abbreviation iteration :: "'a predT \<Rightarrow> 'a predT" ("_\<^sup>\<star>" [1000] 1000) where
   "F\<^sup>\<star> \<equiv> near_quantale_unital.qstar Sup op \<circ> id F"
 
 definition if_comm :: "'a pred \<Rightarrow> 'a predT \<Rightarrow> 'a predT \<Rightarrow> 'a predT" where
@@ -185,6 +183,7 @@ syntax
   "_antiquote_h" :: "('a \<Rightarrow> 'b) \<Rightarrow> 'a" ("|_|" [1000] 1000) (* Apply heap *)
   "_assign" :: "idt \<Rightarrow> 'b \<Rightarrow> 'a predT" ("(`_ :=/ _)" [70, 65] 61)
   "_mutation" :: "'b \<Rightarrow> 'b \<Rightarrow> 'a predT" ("(@_ :=/ _)" [70, 65] 61)
+  "_subst" :: "'a pred \<Rightarrow> 'b \<Rightarrow> idt \<Rightarrow> 'a pred" ("_[_'/`_]" [1000] 999)
   "_if" :: "'a pred \<Rightarrow> 'a predT \<Rightarrow> 'a predT \<Rightarrow> 'a predT" ("(0if _//then _//else _//fi)" [0,0,0] 61)
   "_if_skip" :: "'a pred \<Rightarrow> 'a predT \<Rightarrow> 'a predT" ("(0if _//then _//fi)" [0,0] 61)
   "_while" :: "'a pred \<Rightarrow> 'a predT \<Rightarrow> 'a predT" ("(0while  _//do _//od)" [0, 0] 61)
@@ -194,6 +193,7 @@ ML_file "while_syntax.ML"
 
 parse_translation {*
   [(@{syntax_const "_quote"}, K quote_tr'),
+    (@{syntax_const "_subst"}, K subst_tr),
     (@{syntax_const "_assign"}, K assign_tr),
     (@{syntax_const "_mutation"}, K mutation_tr),
     (@{syntax_const "_if"}, K if_tr), 
@@ -203,5 +203,97 @@ parse_translation {*
 
 translations
   "if b then x fi" == "if b then x else skip fi"
+
+(* Syntactic sugar of predicates about heap *)
+syntax
+  "_is_singl" :: "nat \<Rightarrow> nat \<Rightarrow> bool" ("_ \<mapsto> _" [56,51] 56)
+  "_ex_singleton" :: "nat \<Rightarrow> bool" ("_ \<mapsto> -" [56] 56)
+  "_is_heap_list" :: "nat \<Rightarrow> nat \<Rightarrow> bool" ("_ [\<mapsto>] _" [56,51] 56)
+
+translations
+  "i \<mapsto> j" == "|(CONST is_singleton i j)|"
+  "i \<mapsto> -" == "|(CONST ex_singleton i)|"
+  "x [\<mapsto>] xs" == "|(`(CONST curry (CONST is_heap_list x xs)))|"
+
+
+section {* Monotonicity *}
+
+text {* All the constructs are monotones. *}
+
+lemma mono_skip: "mono skip"
+  by (simp add: mono_def)
+
+lemma mono_assign: "mono ( `x := ` |m| )"
+  by (auto simp: mono_def)
+
+lemma mono_mutation: "mono ( @`x := `m )"
+  by (auto simp: mono_def)
+
+lemma mono_seq: "mono F \<Longrightarrow> mono G \<Longrightarrow> mono (F o G)"
+  by (auto simp: mono_def)
+
+lemma mono_if: "mono F \<Longrightarrow> mono G \<Longrightarrow> mono (if_comm p F G)"
+  by (auto simp: if_comm_def mono_def)
+
+lemma mono_iteration: "mono F \<Longrightarrow> mono F\<^sup>\<star>"
+  apply (simp add: mono_def)
+  apply clarify
+sorry
+
+lemma mono_while: "mono F \<Longrightarrow> mono (while_comm p F)"
+  apply (auto simp: while_comm_def intro!: mono_seq mono_iteration)
+  by (auto simp: mono_def)
+
+section {* Locality *}
+
+definition local :: "'a predT \<Rightarrow> bool" where
+  "local F \<equiv> \<forall>x y. F x * y \<le> F (x * y)"
+
+text {* All the constructs are local *}
+
+lemma local_skip: "local skip"
+  by (simp add: local_def)
+
+lemma local_seq: "mono F \<Longrightarrow> local F \<Longrightarrow> local G \<Longrightarrow> local (F o G)"
+proof (subst local_def, (rule allI)+, (subst comp_apply)+)
+  fix x y assume assms: "mono F" "local F" "local G"
+  hence "F (G x) * y \<le> F (G x * y)"
+    by (simp add: local_def)
+  also have "... \<le> F (G (x * y))" using assms
+    by (auto simp add: assms local_def mono_def)
+  finally show "F (G x) * y \<le> F (G (x * y))" .
+qed
+
+lemma local_if: "local F \<Longrightarrow> local G \<Longrightarrow> local (if_comm p F G)"
+  by (auto simp: if_comm_def local_def)
+
+lemma local_power: "mono F \<Longrightarrow> local F \<Longrightarrow> local (near_quantale_unital.qpower op \<circ> skip F i)"
+  apply (induct i)
+  by (auto simp: local_skip intro: local_seq)
+
+lemma local_sup: "local f \<Longrightarrow> local g \<Longrightarrow> local (f \<squnion> g)"
+proof (subst local_def, (rule allI)+, simp)
+  fix x y assume assms: "local f" "local g"
+  have "(f x \<squnion> g x) * y \<le> f x * y \<squnion> g x * y"
+    by (metis Semantics.Sup.qdistr eq_refl)
+  also have "... \<le>  f (x * y) \<squnion> g (x * y)" using assms
+    apply (unfold local_def)
+    by (metis sup.mono)
+  finally show "(f x \<squnion> g x) * y \<le> f (x * y) \<squnion> g (x * y)" .
+qed
+
+lemma local_Sup: "\<forall>f \<in> F. local f \<Longrightarrow> local (\<Squnion>f)"
+  sorry
+
+lemma local_iteration: "mono F \<Longrightarrow> local F \<Longrightarrow> local F\<^sup>\<star>"
+  apply (simp add: PT.Sup.qstar_def)
+  apply (rule local_Sup[of "{y. \<exists>i. y = near_quantale_unital.qpower op \<circ> skip F i}"])
+  by (auto intro: local_power)
+
+lemma local_while: "mono F \<Longrightarrow> local (op \<squnion> p) \<Longrightarrow> local F \<Longrightarrow> local (while_comm p F)"
+  apply (simp add: while_comm_def)
+  apply (auto intro!: local_seq local_iteration mono_iteration mono_seq)
+  apply (auto simp: mono_def)
+oops
 
 end
