Tool/Examples.thy
@@ -1,0 +1,55 @@
+theory Examples
+  imports Hoare GCD
+begin
+
+no_notation Set.image (infixr "`" 90)
+  and times (infixl "*" 70)
+
+record state =
+  x :: nat
+  y :: nat
+  z :: nat
+  w :: nat
+
+(* Assignments *)
+lemma "\<turnstile> true (`x := 2) \<lbrace> `x = 2 \<rbrace>"
+  by hoare auto
+
+(* Sequential composition *)
+lemma swap: 
+  "\<turnstile> \<lbrace> `x = xo \<and> `y = yo \<rbrace> (
+    `z := `x;
+    `x := `y;
+    `y := `z
+  ) \<lbrace> `x = yo \<and> `y = xo \<rbrace>"
+  by hoare auto
+
+(* If statement *)
+lemma maximum: "\<turnstile> true (if `x \<ge> `y then `z := `x else `z := `y fi) \<lbrace> `z = max `x `y \<rbrace>"
+  by hoare auto
+
+(* While statement *)
+lemma euclids:
+  "\<turnstile> \<lbrace> `x = xo \<and> `y = yo \<rbrace> (
+    while `y \<noteq> 0 
+    inv \<lbrace> gcd `x `y = gcd xo yo \<rbrace>
+    do
+      `z := `y;
+      `y := `x mod `y;
+      `x := `z
+    od
+  ) \<lbrace> `x = gcd xo yo \<rbrace>"
+  by (hoare, auto) (metis gcd_red_nat)
+
+(* Pointers *)
+lemma "\<turnstile> (\<lbrace> `x \<mapsto> `y \<rbrace> * \<lbrace> `z \<mapsto> `w \<rbrace>) skip \<lbrace> `x \<noteq> `z \<rbrace>"
+  by hoare (auto simp: sep_conj_def ortho_def is_singleton_def)
+
+lemma "emp * emp \<le> skip emp"
+  by (auto simp: emp_def sep_conj_def ortho_def)
+
+lemma "\<lbrace> `x \<mapsto> `y \<rbrace> * \<lbrace> `z \<mapsto> `w \<rbrace> \<le> (`y := `w) \<lbrace> `x \<noteq> `z \<rbrace>"
+  by (auto simp: sep_conj_def ortho_def is_singleton_def)
+
+hide_const x y z w
+end
