Tool/Hoare.thy
@@ -1,0 +1,93 @@
+theory Hoare
+  imports Semantics
+begin
+
+definition ht :: "'a pred \<Rightarrow> 'a predT \<Rightarrow> 'a pred \<Rightarrow> bool" ("(3\<turnstile> _/ (2_)/ _)" [100, 55, 100] 50) where
+  "\<turnstile> p F q \<longleftrightarrow> p \<le> F q"
+
+lemma hl_seq: "mono F \<Longrightarrow> \<turnstile> r G q \<Longrightarrow> \<turnstile> p F r \<Longrightarrow> \<turnstile> p F; G q"
+  by (auto simp: ht_def mono_def)
+
+lemma hl_skip: "p \<le> q \<Longrightarrow> \<turnstile> p skip q"
+  by (auto simp: ht_def)
+
+lemma hl_if: "\<turnstile> (p \<sqinter> b) F q \<Longrightarrow> \<turnstile> (p - b) G q \<Longrightarrow> \<turnstile> p (if_comm b F G) q"
+  by (auto simp: ht_def if_comm_def)
+
+lemma hl_weaken: "mono F \<Longrightarrow> q \<le> q' \<Longrightarrow> \<turnstile> p F q \<Longrightarrow> \<turnstile> p F q'"
+  by (auto simp: ht_def mono_def)
+
+lemma hl_strenthen: "p' \<le> p \<Longrightarrow> \<turnstile> p F q \<Longrightarrow> \<turnstile> p' F q"
+  by (auto simp: ht_def)
+
+lemma iteration: "p \<le> F q \<Longrightarrow> p \<le> F\<^sup>\<star> q"
+proof -
+  assume assm: "p \<le> F q"
+  have "F \<le> F\<^sup>\<star>"
+    by (metis PT.Sup.qpower.simps PT.Sup.qstar_refi comp_id)
+  thus ?thesis using assm
+    by force
+qed
+
+lemma hl_while: "mono x \<Longrightarrow> p \<le> i \<Longrightarrow> i - b \<le> q \<Longrightarrow> (i \<sqinter> b) \<le> x i \<Longrightarrow> \<turnstile> p (while_inv_comm b i x) q"
+  apply (simp add: ht_def while_inv_comm_def)
+  apply (auto intro!: iteration )
+  apply (rule rev_predicate1D[of "\<lambda>s. x i s"])
+  prefer 2
+  apply (rule monoD[of x])
+  by auto
+
+lemma sl_frame: "local F \<Longrightarrow> \<turnstile> p F q \<Longrightarrow> \<turnstile> (p * r) F (q * r)"
+proof (simp add: local_def ht_def)
+  assume assm: "\<forall>x y. F x * y \<le> F (x * y)" "p \<le> F q"
+  hence "p * r \<le> F q * r"
+    by (metis Semantics.Sup.qisor)
+  thus "p * r \<le> F (q * r)" using assm
+    by auto
+qed
+
+lemma hl_assign: "P \<le> Q[` |m| /`x] \<Longrightarrow> \<turnstile> P (`x := ` |m| ) Q"
+  by (auto simp: ht_def)
+
+lemma sl_mutation: "P \<le> \<lbrace>`x \<mapsto> -\<rbrace> * (\<lbrace> `x \<mapsto> `m \<rbrace> -* Q) \<Longrightarrow> \<turnstile> P (@`x := `m) Q"
+  sorry
+
+ML {*
+
+val hoare_step_tac = 
+  resolve_tac [
+      @{thm order_refl},
+      @{thm mono_seq},
+      @{thm mono_assign},
+      @{thm mono_mutation},
+      @{thm hl_assign}, 
+      @{thm sl_mutation},
+      @{thm hl_if}, 
+      @{thm hl_skip}, 
+      @{thm hl_seq},
+      @{thm hl_while}
+    ] 
+
+val hoare_tac = REPEAT_ALL_NEW (CHANGED o hoare_step_tac)
+
+*}
+
+method_setup hoare_simp = {*
+  Scan.succeed (fn ctxt => SIMPLE_METHOD (
+    ALLGOALS hoare_tac 
+    THEN ALLGOALS (asm_full_simp_tac ctxt)
+  ))
+*}
+
+method_setup hoare_step = {*
+  Scan.succeed (fn ctxt => SIMPLE_METHOD (
+    ALLGOALS hoare_step_tac 
+  ))
+*}
+
+method_setup hoare = {*
+  Scan.succeed (fn ctxt => SIMPLE_METHOD (
+    ALLGOALS hoare_tac
+  ))
+*}
+end
